More properties of zip trees (thanks Wouter)

theories/zip.v
@@ -1,4 +1,4 @@
-(* Copyright (c) 2023 Microsoft Research, Anton Lorenzen, Wouter Swierstra *)
+(* Copyright (c) 2023 Wouter Swierstra, Microsoft Research, Anton Lorenzen *)
 
 From Equations Require Import Equations.
 From fip_iris Require Import lang.
@@ -42,8 +42,9 @@ Fixpoint smaller (i : Z) (t : tree) : tree :=
   | Node rk l x r =>
     if bool_decide (x < i)%Z then
       Node rk l x (smaller i r)
-    else
+    else if bool_decide (x > i)%Z then
       smaller i l
+    else l
   end.
 
 Fixpoint bigger (i : Z) (t : tree) : tree :=
@@ -52,19 +53,21 @@ Fixpoint bigger (i : Z) (t : tree) : tree :=
   | Node rk l x r =>
     if bool_decide (x < i)%Z then
       bigger i r
-    else
+    else if bool_decide (x > i)%Z then
       Node rk (bigger i l) x r
+    else r
   end.
 
 Fixpoint rec_insert (i : Z) (rank : Z) (t : tree) : tree :=
   match t with
   | Node rnk l x r =>
     if is_higher_rank rnk rank x i
-      then if bool_decide (x < i)%Z
-        then Node rnk l x (rec_insert i rank r)
-        else Node rnk (rec_insert i rank l) x r
-      else if bool_decide (x = i)%Z then t
-      else Node rank (smaller i t) i (bigger i t) 
+    then if bool_decide (x < i)%Z
+         then Node rnk l x (rec_insert i rank r)
+         else Node rnk (rec_insert i rank l) x r
+    else if bool_decide (x = i)%Z
+         then t
+         else Node rank (smaller i t) i (bigger i t) 
   | Leaf => Node rank (smaller i t) i (bigger i t) 
   end.
 
@@ -244,32 +247,630 @@ Definition td_insert (t : tree) (rank : Z) (k : Z) : tree :=
 
 Local Hint Unfold td_insert td_insert_go : trees.
 
+(* Properties of zip trees *)
+
+Inductive all (P : Z -> Type) : tree -> Type :=
+| all_leaf : all P Leaf
+| all_node : forall {l : tree} {rnk x : Z} {r : tree},
+             all P l -> P x -> all P r -> all P (Node rnk l x r).
+
+Local Hint Constructors all : trees.
+
+Lemma all_impl {P Q : Z → Set} {t : tree} (H : all P t) (f : forall x : Z, P x → Q x) : all Q t.
+Proof.
+  induction t; [ now trivial with trees | ].
+  inversion H; now auto with trees.
+Qed.
+
+Local Hint Resolve all_impl : trees.
+Local Hint Unfold insert : trees.
+Inductive in_tree (x rank : Z) : tree -> Type :=
+  | in_root : forall {l r : tree}, in_tree x rank (Node rank l x r)
+  | in_left : forall {l r : tree} {y rnk : Z},
+      in_tree x rank l -> in_tree x rank (Node rnk l y r)
+  | in_right : forall {l r : tree} {y rnk : Z},
+      in_tree x rank r -> in_tree x rank (Node rnk l y r).
+
+Local Hint Constructors in_tree : trees.
+
+Lemma in_tree_all (P : Z -> Type) {t : tree} {x rank : Z} :
+  in_tree x rank t -> all P t -> P x.
+  Proof.  
+  induction t as [ | rnk l IHl k r IHr].
+  - intros H; now inversion H.
+  - intros elem allP; inversion elem; inversion allP; subst; try assumption.
+    + now apply IHl.
+    + now apply IHr.
+Qed.
+
+Lemma smaller_all {P : Z -> Type} {k : Z} {t : tree} :
+  all P t -> all P (smaller k t).
+  intro H; induction t as [ | rnk l IHl x r IHr]; [now constructor | ].
+  inversion H; unfold smaller; case_bool_decide; subst.
+  - constructor; try assumption. fold smaller. now apply IHr.
+  - fold smaller. case_bool_decide.
+    * now apply IHl.
+    * assumption.
+Qed.
+
+Lemma bigger_all {P : Z -> Type} {k  : Z} {t : tree} :
+  all P t -> all P (bigger k t).
+  intro H; induction t as [ | rnk l IHl x r IHr]; [now constructor | ].
+  inversion H; unfold bigger; case_bool_decide; subst.
+  - fold bigger; now apply IHr.
+  - case_bool_decide; fold bigger.
+    + constructor; [ now apply IHl | assumption | assumption ].
+    + assumption.
+Qed.
+
+Local Hint Resolve smaller_all bigger_all : trees.
+
+Lemma rec_insert_all {P : Z -> Type} {k rank : Z} {t : tree} :
+  all P t -> P k -> all P (rec_insert k rank t).
+Proof.
+intros H pk; induction t as [ | rnk l IHl x r IHr].
+- inversion H; constructor; trivial.
+- inversion H; unfold rec_insert.
+  destruct (is_higher_rank rnk rank x k).
+  case_bool_decide; fold rec_insert.
+  + constructor; try assumption; now apply IHr.
+  + constructor; try assumption; now apply IHl.
+  + case_bool_decide.
+    * constructor;  assumption.
+    * repeat constructor; try assumption.
+      all: try apply smaller_all; try assumption.
+      all: apply bigger_all; try assumption.
+Qed.
+
+Local Hint Resolve rec_insert_all : trees.
+
+Inductive is_bst : tree -> Type :=
+| is_bst_leaf : is_bst Leaf
+| is_bst_node : forall {x rnk : Z} {l r : tree},
+    is_bst l -> all (fun y => Z.le y x) l ->
+    is_bst r -> all (fun y => Z.lt x y) r ->
+    is_bst (Node rnk l x r).
+
+Local Hint Constructors is_bst : trees.
+
+Lemma smaller_bst (t : tree) (k : Z) (bst_t : is_bst t) 
+   : is_bst (smaller k t).
+Proof.
+  induction t as [ | rnk l IHl x r IHr].
+  - constructor.
+  - unfold smaller; case_bool_decide; fold smaller.
+    * inversion bst_t; constructor; subst; try assumption.
+      + now apply IHr.
+      + now apply smaller_all.
+    * inversion bst_t; subst; case_bool_decide.
+      + now apply IHl.
+      + assumption.
+Qed.      
+
+Lemma smaller_is_smaller (t : tree) (k : Z) (bst_t : is_bst t) :
+  all (fun y => Z.le y k) (smaller k t).
+  Proof.
+    induction t as [ | rnk l IHl x r IHr].
+    - constructor.
+    - unfold smaller; case_bool_decide; fold smaller.
+      * inversion bst_t as [ | x' rnk' l' r' bst_l all_l bst_r all_r ]; subst.
+        constructor; [ apply (all_impl all_l); simpl; lia | lia | ].
+        now apply IHr.
+      * inversion bst_t; case_bool_decide; [ now apply IHl | ].
+        assert (x = k) by lia; subst; assumption.
+  Qed.
+
+Local Hint Resolve smaller_bst smaller_is_smaller : trees.
+  
+Lemma bigger_bst (t : tree) (k : Z) (bst_t : is_bst t) 
+   : is_bst (bigger k t).
+  induction t as [ | rnk l IHl x r IHr].
+  - constructor.
+  - unfold bigger; case_bool_decide; fold bigger.
+    * inversion bst_t; subst.
+      now apply IHr.
+    * case_bool_decide.
+      + inversion bst_t; constructor; subst; try assumption.
+        now apply IHl.
+        now apply bigger_all.
+      + inversion bst_t; assumption.
+Qed.
+
+Lemma bigger_is_bigger ( t : tree) (k : Z) (bst_t : is_bst t) :
+  all (fun y => Z.lt k y) (bigger k t).
+  Proof.
+    induction t as [ | rnk l IHl x r IHr].
+    - constructor.
+    - unfold bigger; case_bool_decide; fold bigger.
+      * inversion bst_t; subst; apply IHr; try assumption.
+      * inversion bst_t as [ | x' rnk' l' r' bst_l all_l bst_r all_r ]; subst.
+        case_bool_decide.
+        + constructor.
+          now apply IHl.
+          destruct (dec_eq x k).
+          ++ lia.
+          ++ lia.
+          ++ apply (all_impl all_r); simpl; intros; lia.
+        + assert (x = k) by lia; subst; assumption.
+  Qed.
+
+Local Hint Resolve bigger_bst bigger_is_bigger : trees.
+
+Lemma bst_left {l r : tree} {rnk rank x y : Z} :
+  is_bst (Node rnk l x r) ->
+  in_tree y rank (Node rnk l x r) ->
+  (Z.le y x)%Z ->
+  sum (in_tree y rank l) (y = x /\ rank = rnk).
+Proof.
+  intros bst inT leq.
+  inversion inT; subst.
+  - right; now split.
+  - now left. 
+  - inversion bst; subst.
+    assert (x < y)%Z.
+    apply (in_tree_all (λ y : Z, (x < y)%Z) H0); try assumption.
+    lia.
+Qed.  
+
+Lemma bst_left_strict {l r : tree} {rnk rank x y : Z} :
+  is_bst (Node rnk l x r) ->
+  in_tree y rank (Node rnk l x r) ->
+  (Z.lt y x)%Z ->
+  (in_tree y rank l).
+Proof.
+  intros bst inT leq.
+  inversion inT; subst.
+  - lia.
+  - assumption.
+  - inversion bst; subst.
+    assert (x < y)%Z.
+    apply (in_tree_all (λ y : Z, (x < y)%Z) H0); try assumption.
+    lia.
+Qed.
+
+Lemma bst_right {l r : tree} {rnk rank x y : Z} :
+  is_bst (Node rnk l x r) ->
+  in_tree y rank (Node rnk l x r) ->
+  (x < y)%Z ->
+  in_tree y rank r.
+  Proof.
+    intros bst elem lt.
+    inversion elem; subst.
+      - lia.
+      - inversion bst; subst.
+        assert (y ≤ x)%Z.
+        now apply (in_tree_all (λ y : Z, (y ≤ x)%Z) H0).
+        lia.
+      - assumption.
+  Qed.
+
+Local Hint Resolve bst_left bst_right : trees.
+  
+Lemma smaller_elem (t : tree) (k y rank : Z) :
+  in_tree y rank t ->
+  (Z.lt y k)%Z ->
+  is_bst t ->
+  in_tree y rank (smaller k t).
+  Proof.
+    intros H lt bst.
+    induction t as [ | rnk l IHl x r IHr]; [ inversion H | ].
+    unfold smaller; case_bool_decide; fold smaller.
+    - inversion H; subst.
+      * constructor.
+      * now apply in_left.
+      * apply in_right. apply IHr; try assumption. now inversion bst.
+    - case_bool_decide.
+      ++ inversion H; subst.
+         assert (x = k) by lia; subst.
+         exfalso; lia.
+         apply IHl; try assumption.
+         inversion bst; assumption.
+         inversion bst; subst.
+         assert (x < y)%Z.
+         apply (in_tree_all (λ y : Z, (x < y)%Z) H3).
+         assumption.
+         lia.
+      ++ assert (x = k) by lia; subst.
+         clear H0; clear H1.
+         destruct (bst_left bst H).
+         lia.
+         assumption.
+         destruct a; lia.
+Qed.
+
+
+Lemma bigger_elem (t : tree) (k y rank : Z) :
+  in_tree y rank t ->
+  (k < y)%Z ->
+  is_bst t ->
+  in_tree y rank (bigger k t).
+  Proof.
+    intros elem lt bst.
+    induction t as [ | rnk l IHl x r IHr]; [ inversion elem | ].
+    unfold bigger; case_bool_decide; fold bigger; subst.
+    - inversion elem; subst.
+      * lia.
+      * inversion bst; subst.
+        assert (y ≤ x)%Z by apply (in_tree_all _ H1 X0).
+        lia.
+      * apply IHr; inversion bst; assumption.
+    - inversion elem; subst; case_bool_decide.
+        + constructor.
+        + exfalso; lia.
+        + apply in_left.
+          apply IHl; inversion bst; assumption.
+        + apply (bst_right bst elem).
+          assert (x = k) by lia.
+          subst; assumption.
+        + now apply in_right.
+        + assumption.
+  Qed.
+
+Local Hint Resolve smaller_elem bigger_elem : trees.
+
+Inductive gt_rank (rank : Z) : tree -> Type :=
+| gt_rank_leaf : gt_rank rank Leaf
+| gt_rank_node : forall {x rnk : Z} {l r : tree},
+    (rank > rnk)%Z ->
+    gt_rank rank (Node rnk l x r).
+
+Inductive ge_rank (rank : Z) : tree -> Type :=
+| ge_rank_leaf : ge_rank rank Leaf
+| ge_rank_node : forall {x rnk : Z} {l r : tree},
+    (rank >= rnk)%Z ->
+    ge_rank rank (Node rnk l x r).
+                                         
+
+Inductive is_zip : tree -> Type :=
+| is_zip_leaf : is_zip Leaf
+| is_zip_node : forall {x rank : Z} {l r : tree},
+    gt_rank rank l ->
+    ge_rank rank r ->
+    is_zip l -> is_zip r -> is_zip (Node rank l x r).
+
+Local Hint Constructors is_zip gt_rank ge_rank : trees.
+
+
+Lemma zip_left : forall rank l x r, is_zip (Node rank l x r) -> is_zip l.
+  intros rank l x r H; now inversion H.
+  Qed.
+
+Lemma zip_right : forall rank l x r, is_zip (Node rank l x r) -> is_zip r.
+  intros rank l x r H; now inversion H.
+  Qed.
+
+Local Hint Resolve zip_left zip_right : trees.
+
+Lemma higher_rank_true {rnk rank x k : Z} :
+   (true = is_higher_rank rnk rank x k) -> (rank ≤ rnk)%Z.
+Proof.
+  unfold is_higher_rank.
+  repeat case_bool_decide; simpl; intros; try lia.
+Qed.  
+
+Lemma higher_rank_false {rnk rank x k : Z} :
+   (false = is_higher_rank rnk rank x k) -> (rank >= rnk)%Z.
+  unfold is_higher_rank.
+  repeat case_bool_decide; simpl; intros; try lia.
+Qed.
+
+Lemma gt_rank_trans {r r' : Z} {t : tree} (gtr : gt_rank r t) :
+  (r <= r')%Z -> gt_rank r' t.
+  inversion gtr; constructor; lia.
+  Qed.
+
+Lemma ge_rank_trans {r r' : Z} {t : tree} (gtr : ge_rank r t) :
+  (r <= r')%Z -> ge_rank r' t.
+  inversion gtr; constructor; lia.
+  Qed.
+
+Lemma unzip_elems (t : tree) (rank rnk k y  : Z) :
+  in_tree y rank t ->
+  is_bst t ->
+  (y ≠ k) ->
+  in_tree y rank
+    (Node rnk (smaller k t) k (bigger k t)).
+  intros inT isBst fresh.
+  induction t as [ | rnk' l IHl x r IHr].
+  - inversion inT.
+  - destruct (Ztrichotomy_inf y k) as [[lt | eq] | gt].
+    + apply in_left.
+      apply smaller_elem; assumption.
+    + subst. exfalso; intuition.
+    + apply in_right; apply bigger_elem; assumption || lia.
+Qed.
+
+Lemma preserves_elems (t : tree) (y k rnk rank : Z) :
+  is_bst t ->
+  (y ≠ k) ->  
+  in_tree y rank t -> in_tree y rank (rec_insert k rnk t).
+  intros bst inT elem; induction t as [ | rnk' l IHl x r IHr]; inversion bst.
+  + inversion elem.
+  + unfold rec_insert.
+    destruct (is_higher_rank rnk' rnk x k); fold rec_insert.
+    - case_bool_decide; inversion elem; subst; eauto with trees.
+    - case_bool_decide; subst; eauto with trees.
+      now apply unzip_elems.
+Qed. 
+
+Local Hint Resolve rec_insert_all smaller_bst smaller_is_smaller
+      bigger_is_bigger bigger_bst : trees.
+
+Lemma rec_insert_bst (t : tree) (k rank : Z) (bst_t : is_bst t)
+  : is_bst (rec_insert k rank t).
+Proof.
+  autounfold with trees. induction t as [ | rnk l IHl x r IHr].
+  - constructor; now eauto with trees.
+  - fold smaller bigger rec_insert in *;
+      destruct (is_higher_rank rnk rank x k).
+    * case_bool_decide; inversion bst_t; subst; constructor; eauto with trees.
+      apply rec_insert_all; assumption || lia.
+    *  case_bool_decide; inversion bst_t; subst; constructor;
+         eauto with trees.
+Qed.
+
+Lemma rec_insert_ge_rank
+      (t : tree) {k rank rnk : Z} :
+      (rank ≤ rnk)%Z -> ge_rank rnk t ->  ge_rank rnk (rec_insert k rank t).
+  intros le_r le_t; induction t as [ | rnk' l IHl x r IHr].
+  constructor; lia.
+  unfold rec_insert.
+  remember (is_higher_rank rnk' rank x k) as b;
+    rename Heqb into rankCmp; destruct b; fold rec_insert.
+  case_bool_decide; inversion le_t; subst; constructor; lia.
+  case_bool_decide; subst; constructor.
+  assert (rank >= rnk')%Z by apply (higher_rank_false rankCmp); now lia.
+  assert (rank >= rnk')%Z by apply (higher_rank_false rankCmp); now lia.
+Qed.
+
+Lemma rec_insert_gt_rank
+      (t : tree) {k rank rnk : Z} :
+  (rnk > rank)%Z ->
+  gt_rank rnk t ->  gt_rank rnk (rec_insert k rank t).
+Proof.  
+  intros gt_r gt_t; induction t as [ | rnk' l IHl x r IHr].
+  + now constructor.
+  + unfold rec_insert; remember (is_higher_rank rnk' rank x k) as b;
+    rename Heqb into rankCmp; destruct b; fold rec_insert.
+    case_bool_decide.
+    - inversion gt_t; subst; constructor; lia.
+    - constructor; unfold is_higher_rank in *; repeat case_bool_decide; try lia.
+      inversion gt_t. lia.
+    - case_bool_decide.
+      ++ constructor.
+         unfold is_higher_rank in *; repeat case_bool_decide; try lia.
+      ++ inversion gt_t;  constructor.
+         unfold is_higher_rank in *; repeat case_bool_decide; try lia.
+Qed.
+
+Lemma gt_rank_smaller {rank k : Z} {t : tree}
+  (gt_t : gt_rank rank t) (zip_t : is_zip t) :
+  gt_rank rank (smaller k t).
+Proof.  
+  induction t as [ | rnk l IHl x r IHr]; [ now constructor | ].
+  unfold smaller; case_bool_decide; fold smaller.
+  inversion gt_t; constructor; subst; try assumption.
+  case_bool_decide; inversion zip_t; inversion gt_t; subst.
+  + apply IHl; try assumption.
+    assert (GT : gt_rank rnk l) by assumption.
+    apply (gt_rank_trans GT); lia.
+  + assert (GT : gt_rank rnk l) by assumption.
+    eapply (gt_rank_trans GT); lia.
+Qed.
+
+Lemma ge_rank_bigger {rank k : Z} {t : tree}
+      (ge_t : ge_rank rank t) (zip_t : is_zip t) :
+  ge_rank rank (bigger k t).
+  induction t as [ | rnk l IHl x r IHr]; [ now constructor | ].
+  unfold bigger; case_bool_decide; fold bigger;
+    inversion ge_t; inversion zip_t; subst.
+  + apply IHr; [ | assumption].
+    assert (GE : ge_rank rnk r) by assumption.
+    apply (ge_rank_trans GE); lia.
+  + case_bool_decide.
+    ++ constructor; lia.
+    ++ assert (GE : ge_rank rnk r) by assumption.
+       apply (ge_rank_trans GE); lia.
+Qed.
+
+Lemma ge_gt  {rank rnk : Z} {t : tree} :
+  gt_rank rank t -> (rnk >= rank)%Z -> ge_rank rnk t.
+  intro H; inversion H; constructor; lia.
+  Qed.
+
+Lemma gt_ge  {rank rnk : Z} {t : tree} :
+  ge_rank rank t -> (rnk > rank)%Z -> gt_rank rnk t.
+  intro H; inversion H; constructor; lia.
+  Qed.
+
+
+Lemma ge_rank_smaller {rank k : Z} {t : tree}
+      (ge_t : ge_rank rank t) (zip_t : is_zip t) :
+  ge_rank rank (smaller k t).
+  induction t as [ | rnk l IHl x r IHr]; [ now constructor | ].
+  unfold smaller; case_bool_decide; fold smaller;
+    inversion ge_t; inversion zip_t; subst.
+  + constructor; assumption.
+  + case_bool_decide.
+    - apply IHl; try assumption.
+      assert (GT : gt_rank rnk l) by assumption.
+      now apply (ge_gt GT).
+    - assert (GT : gt_rank rnk l) by assumption.
+      assert (GE : ge_rank rnk l) by (apply (ge_gt GT); lia).
+      apply (ge_rank_trans GE); lia.
+Qed.
+
+Lemma gt_rank_bigger {rank k : Z} {t : tree}
+      (gt_rank_t : gt_rank rank t) (zip_t : is_zip t) :
+      gt_rank rank (bigger k t).
+Proof.
+  induction t as [ | rnk l IHl x r IHr]; [ now constructor | ].
+  unfold bigger; case_bool_decide; fold bigger;
+   inversion gt_rank_t; inversion zip_t; subst.
+  - apply IHr; try assumption.
+    assert (GE : ge_rank rnk r) by assumption.
+    now apply (gt_ge GE).
+  - case_bool_decide.
+    ++ constructor; assumption.
+    ++ assert (GE : ge_rank rnk r) by assumption.
+       now (apply (gt_ge GE)).
+Qed.
+
+Lemma smaller_zips {k : Z} {t : tree}
+      (zip_t : is_zip t) : is_zip (smaller k t).
+Proof.
+  induction t as [ | rank l IHl x r IHr]; [ now constructor | ].
+  unfold smaller; case_bool_decide; fold smaller.
+  + constructor; inversion zip_t; subst; eauto with trees.
+    now apply ge_rank_smaller.
+  +  case_bool_decide; inversion zip_t.
+    - now apply IHl. 
+    - assumption.
+Qed.
+
+Lemma bigger_zips {k : Z} {t : tree} (zip_t : is_zip t)  :
+  is_zip (bigger k t).
+Proof.
+  induction t as [ | rank l IHl x r IHr]; [ now constructor | ].
+  unfold bigger; case_bool_decide; fold bigger; inversion zip_t; subst.
+  + now apply IHr.
+  + case_bool_decide; try assumption.
+    constructor; try assumption.
+      ++ apply gt_rank_bigger; try assumption.
+      ++ apply IHl; assumption.
+Qed.
+
+Lemma rec_insert_zip
+      (t : tree) (k rank : Z) (zip_t : is_zip t) 
+  : is_zip (rec_insert k rank t).
+  autounfold with trees; induction t as [ | rnk l IHl x r IHr].
+  - constructor; now eauto with trees.
+  - fold smaller bigger rec_insert in *.
+    remember (is_higher_rank rnk rank x k) as b;
+      rename Heqb into rankCmp; destruct b.
+    + case_bool_decide; inversion zip_t; subst.
+      * constructor; try assumption.
+        ++ apply rec_insert_ge_rank; try assumption.
+           now apply (higher_rank_true rankCmp).
+        ++ apply IHr.
+           assumption.
+      * constructor; try assumption.
+        ++ apply rec_insert_gt_rank; try assumption.
+           unfold is_higher_rank in rankCmp; repeat case_bool_decide; lia.
+        ++ apply IHl.
+           assumption.
+    + case_bool_decide; inversion zip_t; subst.
+      * constructor; try assumption.
+      * constructor.
+        ++ assert (rank >= rnk)%Z by (apply (higher_rank_false rankCmp)).
+           unfold smaller; case_bool_decide; fold smaller.
+           unfold is_higher_rank in rankCmp; simpl in rankCmp.
+           assert (rnkLeRank : (rnk ≤ rank)%Z) by lia.
+           destruct (Z_le_lt_eq_dec _ _ rnkLeRank).
+           constructor; try lia; subst.
+           case_bool_decide; inversion rankCmp.
+           case_bool_decide; inversion rankCmp.
+           case_bool_decide.
+           exfalso; now intuition.
+           exfalso; now intuition.
+           exfalso; now intuition.
+           case_bool_decide.
+           +++ apply gt_rank_smaller.
+           assert (gt_rank rnk l) as GTRankL by assumption.
+           apply (gt_rank_trans GTRankL); now lia. 
+           assumption.
+           +++ assert (x = k) by lia; contradiction.
+        ++ apply ge_rank_bigger; constructor; try assumption.
+           assert (rank >= rnk)%Z by (apply (higher_rank_false rankCmp)).
+           trivial.
+        ++ now apply smaller_zips.
+        ++ now apply bigger_zips.
+Qed.
+
+Lemma ranks_non_increasing_ge {t : tree} {k rnk rank : Z} :
+  is_zip t -> ge_rank rank t -> in_tree k rnk t -> (rnk <= rank)%Z.
+Proof.
+  induction t.
+  - intros. inversion H1.
+  - intros. inversion H1.
+    + subst. inversion H0. lia.
+    + inversion H; subst. assert (ge_rank rank t1).
+      apply (ge_gt H11). now inversion H0. now apply IHt1.
+    + inversion H; subst. inversion H0. assert (ge_rank rank t2).
+      apply (ge_rank_trans H12). lia. now apply IHt2. 
+Qed.
+
+Lemma ranks_non_increasing_gt {t : tree} {k rnk rank : Z} :
+  is_zip t -> gt_rank rank t -> in_tree k rnk t -> (rnk < rank)%Z.
+Proof.
+  induction t.
+  - intros. inversion H1.
+  - intros. inversion H1.
+    + subst. inversion H0. lia.
+    + inversion H; subst. inversion H0. assert (gt_rank rank t1).
+      apply (gt_rank_trans H11). lia. now apply IHt1.
+    + inversion H; subst. inversion H0. assert (gt_rank rank t2).
+      inversion H12. now apply gt_rank_leaf. apply gt_rank_node. lia.
+      now apply IHt2.
+Qed.
+
+Lemma fresh_key_below_correct_rank (x i rank rk : Z) (t1 t2 : tree)
+  (zt : is_zip (Node rk t1 x t2)) (bt : is_bst (Node rk t1 x t2))
+  (rankFromKey : ∀ rk0 : Z, in_tree i rk0 (Node rk t1 x t2) → rk0 = rank)
+  (H : x ≠ i) (H0 : is_higher_rank rk rank x i = false)
+  : forall x0 rk0, in_tree x0 rk0 (Node rk t1 x t2) -> x0 ≠ i.
+Proof.
+  intros. intro. subst. assert (rk0 = rank) by now apply (rankFromKey rk0).
+  inversion H1.
+  - lia.
+  - inversion zt.
+    assert (rk0 < rk)%Z by apply (ranks_non_increasing_gt H14 H12 H4).
+    unfold is_higher_rank in H0. repeat case_bool_decide; try lia.
+  - inversion zt. assert (rk0 <= rk)%Z by apply (ranks_non_increasing_ge H15 H13 H4).
+    unfold is_higher_rank in H0. repeat case_bool_decide; try lia.
+    subst. inversion bt. assert (x < i)%Z by apply (in_tree_all (λ y : Z, (x < y)%Z) H4 X2).
+    contradiction.
+Qed.
+
 (* Proof of equivalence *)
 
-Lemma smaller_bigger_is_bu_unzip (i : Z) : forall t z1 z2,
+Lemma smaller_bigger_is_bu_unzip (i : Z) (t : tree)
+  (freshKey : (forall x rk, in_tree x rk t -> x ≠ i)) : forall z1 z2,
   (rebuild z1 (smaller i t), rebuild z2 (bigger i t)) = bu_unzip t i z1 z2.
 Proof.
   induction t; unfold smaller; unfold bigger; unfold bu_unzip. reflexivity. case_bool_decide.
   - fold bu_unzip. intros. rewrite <- IHt2. reflexivity.
-  - fold bu_unzip. intros. rewrite <- IHt1. reflexivity.
+    intros. apply (freshKey x0 rk0). now apply in_right.
+  - fold bu_unzip. case_bool_decide.
+    + intros. rewrite <- IHt1. reflexivity.
+      intros. apply (freshKey x0 rk0). now apply in_left.
+    + exfalso. apply (freshKey x rk). now apply in_root. lia.
 Qed.
 
-Lemma rec_is_bu_go (i rank : Z) : forall t z,
-  rebuild z (rec_insert i rank t) = bu_insert_go t rank i z.
+Lemma rec_is_bu_go (i rank : Z) (t : tree) (zt : is_zip t) (bt : is_bst t)
+  (rankFromKey : (forall rk, in_tree i rk t -> rk = rank))
+  : forall z, rebuild z (rec_insert i rank t) = bu_insert_go t rank i z.
 Proof.
   induction t; autounfold with trees. reflexivity.
-  destruct (is_higher_rank rk rank x i).
+  case_eq (is_higher_rank rk rank x i).
   - case_bool_decide.
     + fold bu_insert_go. intros. rewrite <- IHt2. reflexivity.
+      now inversion zt. now inversion bt.
+      intros. apply (rankFromKey rk0). now apply in_right.
     + fold bu_insert_go. intros. rewrite <- IHt1. reflexivity.
+      now inversion zt. now inversion bt.
+      intros. apply (rankFromKey rk0). now apply in_left.
   - case_bool_decide.
     + reflexivity.
-    + rewrite <- smaller_bigger_is_bu_unzip. reflexivity.
+    + intros. rewrite <- smaller_bigger_is_bu_unzip. reflexivity.
+      now apply (fresh_key_below_correct_rank x i rank rk).
 Qed.
 
-Lemma rec_is_bu (i rank : Z) (t : tree) : rec_insert i rank t = bu_insert t rank i.
+Lemma rec_is_bu (i rank : Z) (t : tree) (zt : is_zip t) (bt : is_bst t)
+  (rankFromKey : (forall rk, in_tree i rk t -> rk = rank))
+  : rec_insert i rank t = bu_insert t rank i.
 Proof.
-  unfold bu_insert. rewrite <- rec_is_bu_go. reflexivity.
+  unfold bu_insert. now rewrite <- rec_is_bu_go.
 Qed.
 
 Lemma td_right_id (i : Z) : forall t z1 z2,
@@ -312,323 +913,47 @@ Proof.
   - fold td_left. rewrite (td_left_id). reflexivity.
 Qed.
 
-Lemma smaller_bigger_is_td_unzip (i : Z) : forall t z1 z2,
+Lemma smaller_bigger_is_td_unzip (i : Z) (t : tree)
+  (freshKey : (forall x rk, in_tree x rk t -> x ≠ i)) : forall z1 z2,
   (plug z1 (smaller i t), plug z2 (bigger i t)) = td_unzip t i z1 z2.
 Proof.
   induction t; unfold smaller; unfold bigger.
   reflexivity. intros. simp td_unzip. case_bool_decide; case_decide; try lia.
   - rewrite (td_right_step H). rewrite <- IHt2. rewrite comp_plug. reflexivity.
-  - rewrite (td_left_step H). rewrite <- IHt1. rewrite comp_plug. reflexivity.
+    intros. apply (freshKey x0 rk0). now apply in_right.
+  - rewrite (td_left_step H). rewrite <- IHt1. rewrite comp_plug. case_bool_decide.
+    + reflexivity.
+    + exfalso. apply (freshKey x rk). now apply in_root. lia.
+    + intros. apply (freshKey x0 rk0). now apply in_left.
 Qed.
 
-Lemma rec_is_td_go (i rank : Z) : forall t z,
-  plug z (rec_insert i rank t) = td_insert_go t rank i z.
+Lemma rec_is_td_go (i rank : Z) (t : tree) (zt : is_zip t) (bt : is_bst t)
+  (rankFromKey : (forall rk, in_tree i rk t -> rk = rank))
+  : forall z, plug z (rec_insert i rank t) = td_insert_go t rank i z.
 Proof.
   induction t; autounfold with trees. reflexivity.
-  destruct (is_higher_rank rk rank x i).
+  case_eq (is_higher_rank rk rank x i).
   - case_bool_decide.
     + fold td_insert_go. intros. rewrite <- IHt2. rewrite comp_plug. reflexivity.
+      now inversion zt. now inversion bt.
+      intros. apply (rankFromKey rk0). now apply in_right.
     + fold td_insert_go. intros. rewrite <- IHt1. rewrite comp_plug. reflexivity.
+      now inversion zt. now inversion bt.
+      intros. apply (rankFromKey rk0). now apply in_left.
   - case_bool_decide.
     + reflexivity.
-    + now rewrite <- smaller_bigger_is_td_unzip.
+    + intros. rewrite <- smaller_bigger_is_td_unzip. reflexivity.
+      now apply (fresh_key_below_correct_rank x i rank rk).
 Qed.
 
-Lemma rec_is_td (i rank : Z) (t : tree) : rec_insert i rank t = td_insert t rank i.
+Lemma rec_is_td (i rank : Z) (t : tree) (zt : is_zip t) (bt : is_bst t)
+  (rankFromKey : (forall rk, in_tree i rk t -> rk = rank))
+  : rec_insert i rank t = td_insert t rank i.
 Proof.
-  unfold td_insert. rewrite <- rec_is_td_go. reflexivity.
+  unfold td_insert. now rewrite <- rec_is_td_go.
 Qed.
 
-Lemma td_is_bu (i rank : Z) (t : tree) : bu_insert t rank i = td_insert t rank i.
+Lemma td_is_bu (i rank : Z) (t : tree) (zt : is_zip t) (bt : is_bst t)
+  (rankFromKey : (forall rk, in_tree i rk t -> rk = rank))
+  : bu_insert t rank i = td_insert t rank i.
 Proof. now rewrite <- rec_is_bu, rec_is_td. Qed.
-
-(* Properties of zip trees *)
-
-(* TODO: fix *)
-
-Inductive all (P : Z -> Type) : tree -> Type :=
-| all_leaf : all P Leaf
-| all_node : forall {l : tree} {rnk x : Z} {r : tree},
-             all P l -> P x -> all P r -> all P (Node rnk l x r).
-
-Local Hint Constructors all : trees.
-
-Lemma all_impl {P Q : Z → Set} {t : tree} (H : all P t) (f : forall x : Z, P x → Q x) : all Q t.
-Proof.
-  induction t; [ now trivial with trees | ].
-  inversion H; now auto with trees.
-Qed.
-
-Local Hint Resolve all_impl : trees.
-Local Hint Unfold insert : trees.
-Inductive in_tree (x : Z) : tree -> Type :=
-  | in_root : forall {l r : tree} {rnk : Z}, in_tree x (Node rnk l x r)
-  | in_left : forall {l r : tree} {y rnk : Z},
-      in_tree x l -> in_tree x (Node rnk l y r)
-  | in_right : forall {l r : tree} {y rnk : Z},
-      in_tree x r -> in_tree x (Node rnk l y r).
-
-Local Hint Constructors in_tree : trees.
-
-Lemma in_tree_all (P : Z -> Type) {t : tree} {x : Z} :
-  in_tree x t -> all P t -> P x.
-  Proof.  
-  induction t as [ | rnk l IHl k r IHr].
-  - intros H; now inversion H.
-  - intros elem allP; inversion elem; inversion allP; subst; try assumption.
-    now apply IHl.
-    now apply IHr.
-  Qed.
-
-Lemma not_in_left {l r : tree} {x rnk k : Z} :
-  (in_tree k (Node rnk l x r) -> False) -> (in_tree k l -> False).
-  intros fresh elem; apply fresh; now apply in_left.
-Qed.  
-
-Lemma not_in_right {l r : tree} {x rnk k : Z} :
-  (in_tree k (Node rnk l x r) -> False) -> (in_tree k r -> False).
-  intros fresh elem; apply fresh; now apply in_right.
-Qed.
-
-Local Hint Resolve not_in_right not_in_left.
-
-Lemma smaller_all {P : Z -> Type} {k : Z} {t : tree} :
-  all P t -> all P (smaller k t).
-  intro H; induction t as [ | rnk l IHl x r IHr]; [now constructor | ].
-  inversion H; unfold smaller; case_bool_decide; subst.
-  - constructor; try assumption. fold smaller. now apply IHr.
-  - fold smaller. now apply IHl.
-  Qed.
-
-Lemma bigger_all {P : Z -> Type} {k  : Z} {t : tree} :
-  all P t -> all P (bigger k t).
-  intro H; induction t as [ | rnk l IHl x r IHr]; [now constructor | ].
-  inversion H; unfold bigger; case_bool_decide; subst.
-  - fold bigger. now apply IHr.
-  - constructor; try assumption. now apply IHl.
-  Qed.
-
-Local Hint Resolve smaller_all bigger_all.
-
-Lemma rec_insert_all {P : Z -> Type} {k rank : Z} {t : tree} :
-  all P t -> P k -> all P (rec_insert k rank t).
-Proof.
-intros H pk; induction t as [ | rnk l IHl x r IHr].
-- inversion H; constructor; trivial.
-- inversion H; unfold rec_insert.
-  destruct (is_higher_rank rnk rank x k).
-  case_bool_decide; fold rec_insert.
-  + constructor; try assumption; now apply IHr.
-  + constructor; try assumption; now apply IHl.
-  + case_bool_decide.
-    * constructor;  assumption.
-    * repeat constructor; try assumption.
-      all: try apply smaller_all; try assumption.
-      all: apply bigger_all; try assumption.
-Qed.
-
-Inductive is_bst : tree -> Type :=
-| is_bst_leaf : is_bst Leaf
-| is_bst_node : forall {x rnk : Z} {l r : tree},
-    is_bst l -> all (fun y => Z.lt y x) l ->
-    is_bst r -> all (fun y => Z.lt x y) r ->
-    is_bst (Node rnk l x r).
-
-Lemma smaller_bst (t : tree) (k : Z) (bst_t : is_bst t) 
-   : is_bst (smaller k t).
-Proof.
-  induction t as [ | rnk l IHl x r IHr].
-  - constructor.
-  - unfold smaller; case_bool_decide; fold smaller.
-    * inversion bst_t; constructor; subst; try assumption.
-      apply IHr; try assumption.
-      now apply smaller_all.
-    * inversion bst_t; subst.
-      now apply IHl.
-Qed.      
-
-Lemma smaller_is_smaller (t : tree) (k : Z) (bst_t : is_bst t) :
-  all (fun y => Z.lt y k) (smaller k t).
-  Proof.
-    induction t as [ | rnk l IHl x r IHr].
-    - constructor.
-    - unfold smaller; case_bool_decide; fold smaller.
-      * inversion bst_t as [ | x' rnk' l' r' bst_l all_l bst_r all_r ]; subst.
-        constructor; [ apply (all_impl all_l); simpl; lia | lia | ].
-        now apply IHr.
-      * inversion bst_t; now apply IHl.
-  Qed.
-
-Lemma bigger_bst (t : tree) (k : Z) (bst_t : is_bst t) 
-   : is_bst (bigger k t).
-  induction t as [ | rnk l IHl x r IHr].
-  - constructor.
-  - unfold bigger; case_bool_decide; fold bigger.
-    * inversion bst_t; subst.
-      now apply IHr.
-    * inversion bst_t; constructor; subst; try assumption.
-      apply IHl; try assumption.
-      now apply bigger_all.
-  Qed.
-
-Lemma bigger_is_bigger ( t : tree) (k : Z) (bst_t : is_bst t)
-  (fresh : (in_tree k t -> False)) :
-  all (fun y => Z.lt k y) (bigger k t).
-  Proof.
-    induction t as [ | rnk l IHl x r IHr].
-    - constructor.
-    - unfold bigger; case_bool_decide; fold bigger.
-      * inversion bst_t; subst; apply IHr; try assumption.
-        intro elem_r; apply fresh; auto with trees.
-      * inversion bst_t as [ | x' rnk' l' r' bst_l all_l bst_r all_r ]; subst.
-        constructor.
-        apply IHl; try assumption.
-        auto with trees.
-        destruct (dec_eq x k).
-        + subst. exfalso. apply fresh; constructor.
-        + lia.
-        + apply (all_impl all_r); simpl; intros; lia.
-  Qed.
-
-Lemma bst_left {l r : tree} {rank x y : Z} :
-  is_bst (Node rank l x r) ->
-  in_tree y (Node rank l x r) ->
-  (y < x)%Z ->
-  in_tree y l.
-  Proof.
-    intros bst elem lt.
-    inversion elem; subst.
-      - lia.
-      - assumption.
-      - inversion bst as [ | a b c d B0 B1 B2 B3]; subst.
-        assert (x < y)%Z by (apply (in_tree_all _ H0); assumption). lia.
-  Qed.
-
-Lemma bst_right {l r : tree} {rank x y : Z} :
-  is_bst (Node rank l x r) ->
-  in_tree y (Node rank l x r) ->
-  (x < y)%Z ->
-  in_tree y r.
-  Proof.
-    intros bst elem lt.
-    inversion elem; subst.
-      - lia.
-      - inversion bst; subst.
-        assert (y < x)%Z.
-        apply (in_tree_all (λ y : Z, (y < x)%Z) H0); assumption.
-        lia.
-      - assumption.
-  Qed.
-  
-Lemma smaller_elem (t : tree) (k y : Z) :
-  in_tree y t ->
-  (y < k)%Z ->
-  is_bst t ->
-  in_tree y (smaller k t).
-  Proof.
-    intros H lt bst.
-    induction t as [ | rnk l IHl x r IHr]; [ inversion H | ].
-    unfold smaller; case_bool_decide; fold smaller.
-    - inversion H; subst.
-      * constructor.
-      * now apply in_left.
-      * apply in_right. apply IHr; try assumption. now inversion bst.
-    - inversion H; subst.
-      * contradiction.
-      * apply IHl; inversion bst; assumption.
-      * inversion bst; subst.
-        assert (x < y)%Z by apply (in_tree_all _ H2 X2).
-        lia.
-   Qed.
-
-Lemma bigger_elem (t : tree) (k y : Z) :
-  in_tree y t ->
-  (k < y)%Z ->
-  is_bst t ->
-  in_tree y (bigger k t).
-  Proof.
-    intros elem lt bst.
-    induction t as [ | rnk l IHl x r IHr]; [ inversion elem | ].
-    unfold bigger; case_bool_decide; fold bigger; subst.
-    - inversion elem; subst.
-      * lia.
-      * inversion bst; subst.
-        assert (y < x)%Z by apply (in_tree_all _ H1 X0).
-        lia.
-      * apply IHr; inversion bst; assumption.
-    - inversion elem; subst.
-      * constructor.
-      * apply in_left.
-        apply IHl; inversion bst; assumption.
-      * now apply in_right.
-  Qed.
-  
-Lemma unzip_elems (t : tree) (rank k y : Z) :
-  in_tree y t  ->
-  is_bst t ->
-  in_tree y (Node rank (smaller k t) k (bigger k t)).
-  Proof.
-    intros inT bst; induction t as [ | rnk l IHl x r IHr]; [now inversion inT | ].
-    destruct (Ztrichotomy_inf k y) as [[lt | eq] | gt].
-    - apply in_right.
-      now apply (bigger_elem).
-    - subst; now constructor.
-    - apply in_left.
-      apply (smaller_elem); try assumption.
-      lia.
-  Qed.
-
-Lemma preserves_elems (t : tree) (y k rank : Z) :
-  is_bst t ->
-  in_tree y t -> in_tree y (rec_insert k rank t).
-  intros bst H; induction t as [ | rnk l IHl x r IHr]; inversion bst.
-  + inversion H.
-  + unfold rec_insert.
-    destruct (is_higher_rank rnk rank x k); fold rec_insert.
-    - case_bool_decide; inversion H; subst.
-      * constructor.
-      * now apply in_left.
-      * apply in_right; now apply IHr.
-      * constructor.
-      * apply in_left; now apply IHl.
-      * now apply in_right. 
-    - case_bool_decide; subst.
-      * assumption.
-      * now apply unzip_elems.
-  Qed. 
-
-  
-Lemma rec_insert_bst (t : tree) (k rank : Z) (bst_t : is_bst t)
-  (fresh : (in_tree k t -> False))
-  : is_bst (rec_insert k rank t).
-Proof.
-  autounfold with trees. induction t as [ | rnk l IHl x r IHr].
-  - constructor; now eauto with trees.
-  - fold smaller bigger rec_insert in *;
-      case_bool_decide; destruct (is_higher_rank rnk rank x k);
-      inversion bst_t; subst.
-    * constructor; try assumption.
-      apply IHr; eauto with trees.
-      now apply rec_insert_all. 
-    * case_bool_decide; [ assumption | ].
-      constructor.
-      now apply smaller_bst.
-      now apply smaller_is_smaller.
-      now apply bigger_bst.
-      now apply bigger_is_bigger.
-    * constructor; try assumption.
-      apply IHl; auto with trees.
-      apply rec_insert_all; try assumption.
-      destruct (dec_eq x k).
-        + subst. exfalso. apply fresh; constructor.
-        + lia.
-    * case_bool_decide; [ assumption | ].
-      constructor.
-      now apply smaller_bst.
-      now apply smaller_is_smaller.
-      now apply bigger_bst.
-      now apply bigger_is_bigger.
-  Qed.
-
-
-
